Remove step parameter from all specs
[step] is a global axiom that avoids reasoning directly about what the
axiomatic primitives inside IO do, which in turn prevent prog from just
being Rets and Binds, which provably don't modify the world state.
There's no need for a semantics of operations over abstract states (and
indeed the parameter was never used, just passed around).

This issued stemmed from fixing Semantics so it is unrelated to the
underlying operations - a Semantics is really just a transition
relation, with a known state and return type, and the global [step] is a
semantics for every (again, axiomatic) primitive operation.

src/Shallow/ProgLang/Hoare.v
@@ -29,8 +29,7 @@ Record Refinement State :=
     abstraction: world -> State }.
 
 Definition prog_spec `(spec: Specification A T State) `(p: prog T)
-           (rf: Refinement State)
-           (step: Semantics State) :=
+           (rf: Refinement State) :=
   forall a w,
     let state := abstraction rf w in
     pre (spec a state) ->
@@ -61,8 +60,7 @@ Definition DoublePre T State :=
 (** [prog_double] defines correctness in terms of a higher-order precondition.
 *)
 Definition prog_double `(pre: DoublePre T State) `(p: prog T)
-           (rf: Refinement State)
-           (step: Semantics State) :=
+           (rf: Refinement State) :=
   forall w postcond crashinv,
     let state := abstraction rf w in
     pre state postcond crashinv ->
@@ -81,8 +79,7 @@ Definition prog_double `(pre: DoublePre T State) `(p: prog T)
 (with separate precondition, postcondition, and crash invariants) into a Hoare
 double. *)
 Definition prog_ok `(spec: Specification A T State) `(p: prog T)
-           (rf: Refinement State)
-           (step: Semantics State) :=
+           (rf: Refinement State) :=
   forall T' (rx: T -> prog T'),
     prog_double
       (fun state postcond crashinv =>
@@ -92,9 +89,9 @@ Definition prog_ok `(spec: Specification A T State) `(p: prog T)
                          post (spec a state) r state' /\
                          postcond' = postcond /\
                          crashinv' = crashinv)
-                      (rx r) rf step) /\
+                      (rx r) rf) /\
               (forall state', crash (spec a state) state' ->
-                     crashinv state')) (Bind p rx) rf step.
+                     crashinv state')) (Bind p rx) rf.
 
 (** We prove a conversion theorem from the Hoare double-based correctness
 statement to the more natural quadruple interpretation. This theorem reveals a
@@ -105,8 +102,7 @@ by the continuation's proof. We cannot make that assumption here when
 establishing the crash invariant in the case that [p] crashes just before
 finishing, so we explicitly assume that the postcondition implies the crash
 invariant. *)
-Theorem prog_ok_to_spec : forall `(step: Semantics State)
-                            `(rf: Refinement State)
+Theorem prog_ok_to_spec : forall `(rf: Refinement State)
                             `(spec: Specification A T State) (p: prog T),
     (forall a w r w',
         let state := abstraction rf w in
@@ -115,7 +111,7 @@ Theorem prog_ok_to_spec : forall `(step: Semantics State)
         post (spec a state) r state' ->
         crash (spec a state) state' /\
         invariant rf w') ->
-    prog_ok spec p rf step -> prog_spec spec p rf step.
+    prog_ok spec p rf -> prog_spec spec p rf.
 Proof.
   unfold prog_ok, prog_double, prog_spec; intros.
   specialize (H0 _ Ret).
@@ -131,10 +127,9 @@ Proof.
   apply monad_right_id; auto.
 Qed.
 
-Theorem prog_spec_to_ok : forall `(step: Semantics State)
-                            `(rf: Refinement State)
+Theorem prog_spec_to_ok : forall `(rf: Refinement State)
                             `(spec: Specification A T State) (p: prog T),
-    prog_spec spec p rf step -> prog_ok spec p rf step.
+    prog_spec spec p rf -> prog_ok spec p rf.
 Proof.
   unfold prog_ok, prog_double, prog_spec; intros.
   deex.
@@ -152,10 +147,9 @@ Proof.
 Qed.
 
 Remark crash_invariants_must_handle_pre :
-  forall `(step: Semantics State)
-    `(rf: Refinement State)
+  forall `(rf: Refinement State)
     `(spec: Specification A T State) (p: prog T),
-    prog_spec spec p rf step ->
+    prog_spec spec p rf ->
     forall a w,
       let state := abstraction rf w in
       pre (spec a state) ->
@@ -169,13 +163,12 @@ Proof.
   apply can_crash_at_begin.
 Qed.
 
-Theorem double_weaken : forall `(step: Semantics State)
-                          `(rf: Refinement State)
+Theorem double_weaken : forall `(rf: Refinement State)
                           T (pre pre': DoublePre T State) (p: prog T),
-    prog_double pre' p rf step ->
+    prog_double pre' p rf ->
     (forall state postcond crashinv, pre state postcond crashinv ->
                             pre' state postcond crashinv) ->
-    prog_double pre p rf step.
+    prog_double pre p rf.
 Proof.
   unfold prog_double at 2; intros.
   eapply H; eauto.
@@ -191,14 +184,13 @@ Definition spec_impl
                (forall state', crash (spec1 a' state) state' ->
                       crash (spec2 a state) state').
 
-Theorem spec_weaken : forall `(step: Semantics State)
-                        `(rf: Refinement State)
+Theorem spec_weaken : forall `(rf: Refinement State)
                         `(spec1: Specification A' T State)
                         `(spec2: Specification A T State)
                         (p: prog T),
-    prog_spec spec1 p rf step ->
+    prog_spec spec1 p rf ->
     forall (Himpl: spec_impl spec1 spec2),
-      prog_spec spec2 p rf step.
+      prog_spec spec2 p rf.
 Proof.
   unfold prog_spec; intros.
   specialize (Himpl a (abstraction rf w)); intuition.
@@ -211,15 +203,14 @@ Proof.
   destruct r; intuition eauto.
 Qed.
 
-Definition ret_ok : forall T (v:T) `(step: Semantics State) `(rf: Refinement State),
+Definition ret_ok : forall T (v:T) `(rf: Refinement State),
     prog_ok
       (fun (_:unit) (state:State) =>
          {| pre := True;
             post := fun r state' => r = v /\ state' = state;
             crash := fun state' => False; |})
       (Ret v)
-      rf
-      step.
+      rf.
 Proof.
   unfold prog_ok, prog_double; intros.
   repeat deex; simpl in *.
@@ -232,12 +223,11 @@ Proof.
   eapply can_crash_at_begin.
 Qed.
 
-Theorem double_exec_equiv : forall `(step: Semantics State)
-                              `(rf: Refinement State)
+Theorem double_exec_equiv : forall `(rf: Refinement State)
                               `(pre: DoublePre T State) (p p': prog T),
     exec_equiv p p' ->
-    prog_double pre p' rf step ->
-    prog_double pre p rf step.
+    prog_double pre p' rf ->
+    prog_double pre p rf.
 Proof.
   unfold prog_double; intros.
   eapply H0 in H1; eauto.
@@ -246,20 +236,20 @@ Qed.
 
 Ltac monad_simpl :=
   repeat match goal with
-         | |- prog_double _ (Bind (Ret _) _) _ _ =>
+         | |- prog_double _ (Bind (Ret _) _) _ =>
            eapply double_exec_equiv; [ apply monad_left_id | ]
-         | |- prog_double _ (Bind (Bind _ _) _) _ _ =>
+         | |- prog_double _ (Bind (Bind _ _) _) _ =>
            eapply double_exec_equiv; [ apply monad_assoc | ]
          end.
 
 (** step_prog_with t handles the first program in a bind by applying tactic t *)
 Ltac step_prog_with t :=
   match goal with
-  | |- prog_double _ _ _ _ =>
+  | |- prog_double _ _ _ =>
     monad_simpl;
     eapply double_weaken; [ solve [ t ] | ]
   | |- forall _, _ => intros; step_prog_with t
-  | |- prog_ok _ _ _ _ => unfold prog_ok; step_prog_with t
+  | |- prog_ok _ _ _ => unfold prog_ok; step_prog_with t
   end.
 
 (** step_prog applies a registered prog_ok theorem (in the prog hint database)
@@ -269,7 +259,7 @@ Ltac step_prog := step_prog_with ltac:(eauto with prog).
 (* This notation builds a pattern; use it as [Hint Extern 1 {{ p; _}} => apply
 p_ok : prog] to associated p_ok as the specification for the program (pattern).
 Such patterns are used by [step_prog] via the prog hint database. *)
-Notation "{{ p ; '_' }}" := (prog_double _ (Bind p _) _ _)
+Notation "{{ p ; '_' }}" := (prog_double _ (Bind p _) _)
                               (only parsing, at level 0).
 
 (** * begin
@@ -282,12 +272,11 @@ haven't made this simplification. *)
 Definition begin := Ret tt.
 Hint Extern 1 {{ begin; _ }} => apply ret_ok : prog.
 
-Lemma begin_prog_ok : forall `(step: Semantics State)
-                        `(rf: Refinement State)
+Lemma begin_prog_ok : forall `(rf: Refinement State)
                         `(spec: Specification A T State)
                         `(p: prog T),
-    prog_ok spec (_ <- begin; p) rf step ->
-    prog_ok spec p rf step.
+    prog_ok spec (_ <- begin; p) rf ->
+    prog_ok spec p rf.
 Proof.
   unfold prog_ok, prog_double; intros.
   repeat deex.
@@ -311,13 +300,12 @@ Ltac intro_begin :=
 (* for programs that are pure the step automation doesn't work, since there is
 no bind in the program *)
 
-Theorem ret_prog_ok : forall `(step: Semantics State)
-                        `(rf: Refinement State)
+Theorem ret_prog_ok : forall `(rf: Refinement State)
                         `(spec: Specification A T State) (v:T),
     (forall a state, pre (spec a state) ->
             post (spec a state) v state /\
             crash (spec a state) state) ->
-    prog_ok spec (Ret v) rf step.
+    prog_ok spec (Ret v) rf.
 Proof.
   intros.
   unfold prog_ok, prog_double; intros.
